NSL: small changes

dolev-yao-star/nsl_pk/NSL.SecurityProperties.fst
@@ -9,28 +9,46 @@ open NSL.Sessions
 
 let is_n_b_in_b_state a b idx_setstate v_b state_b idx_sess n_b =
   state_was_set_at idx_setstate b v_b state_b /\
-  state_inv nsl idx_setstate b v_b state_b /\
   idx_sess < Seq.length state_b /\
-  (match parse_session_st (state_b.[idx_sess]) with
-  |Success (ResponderSentMsg2 a' n_a n_b') -> n_b==n_b' /\ a = a'
-  |Success (ResponderReceivedMsg3 a' n_b') -> n_b==n_b' /\ a = a'
-  |_ -> False
+  (match LabeledPKI.parse_session_st (state_b.[idx_sess]) with
+  | Success (APP s) -> (
+    match NSL.Sessions.parse_session_st s with
+    | Success (ResponderReceivedMsg3 a' n_b') -> n_b==n_b' /\ a = a'
+    | _ -> False
+  )
+  | _ -> False
   )
 
 
-let n_b_is_secret n_b = secrecy_lemma #(pki nsl) n_b
+let n_b_is_secret a b idx_setstate v_b state_b idx_sess n_b =
+  let t0= get () in
+  assert(valid_trace (pki nsl) t0);
+  assert(idx_setstate < trace_len t0);
+  assert(is_n_b_in_b_state a b idx_setstate v_b state_b idx_sess n_b);
+  assert(state_inv (pki nsl) idx_setstate b v_b state_b);
+  assert(is_labeled (pki nsl).global_usage (idx_setstate) n_b (readers ([P a; P b])));
+  assert(later_than (trace_len t0) idx_setstate);
+  assert(is_labeled (pki nsl).global_usage (trace_len t0) n_b (readers ([P a; P b])));
+  secrecy_lemma #(pki nsl) n_b
 
 
 let is_n_b_in_a_state a b idx_setstate v_a state_a idx_sess n_b =
   state_was_set_at idx_setstate a v_a state_a /\
-  state_inv nsl idx_setstate a v_a state_a /\
   idx_sess < Seq.length state_a /\
-  (match parse_session_st (state_a.[idx_sess]) with
-  |Success (InitiatorSentMsg3 b' n_a n_b') -> n_b==n_b' /\ b=b'
-  |_ -> False
+  (match LabeledPKI.parse_session_st (state_a.[idx_sess]) with
+  | Success (APP s) -> (
+    match NSL.Sessions.parse_session_st s with
+    |Success (InitiatorSentMsg3 b' n_a n_b') -> n_b==n_b' /\ b=b'
+    | _ -> False
+  )
+  | _ -> False
   )
 
-let n_b_in_a_state_is_secret n_b = secrecy_lemma #(pki nsl) n_b
+
+let n_b_in_a_state_is_secret a b idx_setstate v_b state_a idx_sess n_b =
+  let t0= get () in
+  assert(later_than (trace_len t0) idx_setstate);
+  secrecy_lemma #(pki nsl) n_b
 
 let initiator_authentication i = ()
 
