dolev-yao-star/nsl_pk/NSL.SecurityProperties.fsti
@@ -23,18 +23,18 @@ val is_n_b_in_b_state:
   state_b:state_vec ->
   idx_sess:nat ->
   n_b:bytes ->
-  Type0 
-  
+  Type0
+
 val n_b_is_secret:
-  #a:principal ->
-  #b:principal ->
-  #idx_setstate:nat ->
-  #v_b:version_vec ->
-  #state_b:state_vec ->
-  #idx_sess:nat ->
+  a:principal ->
+  b:principal ->
+  idx_setstate:nat ->
+  v_b:version_vec ->
+  state_b:state_vec ->
+  idx_sess:nat ->
   n_b:bytes ->
   LCrypto unit (pki nsl)
-  (requires fun t0 -> idx_setstate <= trace_len t0 /\ is_n_b_in_b_state a b idx_setstate v_b state_b idx_sess n_b)
+  (requires fun t0 -> idx_setstate < trace_len t0 /\ is_n_b_in_b_state a b idx_setstate v_b state_b idx_sess n_b)
   (ensures fun t0 _ t1 -> t0 == t1 /\
     (is_unknown_to_attacker_at (trace_len t0) n_b \/
      contains_corrupt_id cpred (trace_len t0) ([P a; P b])))
@@ -50,15 +50,15 @@ val is_n_b_in_a_state:
   Type0
 
 val n_b_in_a_state_is_secret:
-  #a:principal ->
-  #b:principal ->
-  #idx_setstate:nat ->
-  #v_a:version_vec ->
-  #state_a:state_vec ->
-  #idx_sess:nat ->
+  a:principal ->
+  b:principal ->
+  idx_setstate:nat ->
+  v_a:version_vec ->
+  state_a:state_vec ->
+  idx_sess:nat ->
   n_b:bytes ->
   LCrypto unit (pki nsl)
-  (requires fun t0 -> idx_setstate <= trace_len t0 /\ is_n_b_in_a_state a b idx_setstate v_a state_a idx_sess n_b)
+  (requires fun t0 -> idx_setstate < trace_len t0 /\ is_n_b_in_a_state a b idx_setstate v_a state_a idx_sess n_b)
   (ensures fun t0 _ t1 -> t0==t1 /\
 		     (is_unknown_to_attacker_at (trace_len t0) n_b \/
 		      contains_corrupt_id cpred (trace_len t0) [P a; P b]))
